cleaned up source defs

src/Source_Definitions.v
@@ -32,112 +32,106 @@ with s_value : trm -> Prop :=
   | s_value_var : forall x, s_value (s_trm_fvar x)
   | s_value_true : s_value s_trm_true
   | s_value_false : s_value s_trm_false
-  | s_value_abs  : forall L T e,
+  | s_value_abs  : forall L s e,
       (forall x, x \notin L -> s_term (s_open_ee_var e x)) ->
-      (s_type T) ->
-      s_value (s_trm_abs T e).
+      (s_type s) ->
+      s_value (s_trm_abs s e).
 
 Scheme s_term_mut := Induction for s_term Sort Prop
 with s_value_mut := Induction for s_value Sort Prop.
 
-Definition s_env := LibEnv.env typ.
+Definition s_ok (G : env_term) : Prop :=
+  ok G /\ forall x s, binds x s G -> s_type s.
 
-(* TODO: s_ok will need to ensure s_type hold on each typ *)
-Inductive s_typing : s_env -> trm -> typ -> Prop :=
-  | s_typing_var : forall G x T,
-      s_ok G -> binds x T G -> s_typing G (s_trm_fvar x) T
+Inductive s_typing : env_term -> trm -> typ -> Prop :=
+  | s_typing_var : forall G x s,
+      s_ok G -> binds x s G -> s_typing G (s_trm_fvar x) s
   | s_typing_true : forall G,
       s_ok G -> s_typing G s_trm_true s_typ_bool
   | s_typing_false : forall G,
       s_ok G -> s_typing G s_trm_false s_typ_bool
-  | s_typing_abs : forall L G e T1 T2,
-      (forall x, x \notin L ->
-        s_typing (G & x ~ T1) (s_open_ee_var e x) T2) ->
-        (s_type T1) ->
-        s_typing G (s_trm_abs T1 e) (s_typ_arrow T1 T2)
-  | s_typing_if : forall G e1 e2 e3 T,
-      s_typing G e1 s_typ_bool -> s_typing G e2 T -> s_typing G e3 T ->
-      s_typing G (s_trm_if e1 e2 e3) T
-  | s_typing_app : forall G e1 e2 T1 T2,
-      s_typing G e1 (s_typ_arrow T1 T2) -> s_typing G e2 T1 ->
-      s_typing G (s_trm_app e1 e2) T2.
-
-(* Santity check theorem. a well-typed source term should have a
- * well-formed source type 
- *)
-Theorem s_typing_implies_s_type : forall G e s,
-  s_typing G e s -> s_type s.
-Proof. (* TODO *)
-Admitted. 
+  | s_typing_abs : forall L G e s1 s2,
+      (forall x, x \notin L -> s_typing (G & x ~ s1) (s_open_ee_var e x) s2) ->
+      (s_type s1) ->
+      s_typing G (s_trm_abs s1 e) (s_typ_arrow s1 s2)
+  | s_typing_if : forall G e1 e2 e3 s,
+      s_typing G e1 s_typ_bool -> s_typing G e2 s -> s_typing G e3 s ->
+      s_typing G (s_trm_if e1 e2 e3) s
+  | s_typing_app : forall G e1 e2 s1 s2,
+      s_typing G e1 (s_typ_arrow s1 s2) -> s_typing G e2 s1 ->
+      s_typing G (s_trm_app e1 e2) s2.
 
 (* contexts *)
 
 Inductive s_eval_context : ctx -> Prop :=
-  | s_eval_context_hole : s_eval_context ctx_hole
+  | s_eval_context_hole : s_eval_context s_ctx_hole
   | s_eval_context_if : forall E e1 e2,
-      s_eval_context E -> s_term e1 -> s_term e2 -> s_eval_context (s_ctx_if E e1 e2)
+      s_eval_context E -> s_term e1 -> s_term e2 ->
+      s_eval_context (s_ctx_if E e1 e2)
   | s_eval_context_app1 : forall E e,
-      s_eval_context E -> s_term e -> s_eval_context (s_ctx_app1 E e)
+      s_eval_context E -> s_term e ->
+      s_eval_context (s_ctx_app1 E e)
   | s_eval_context_app2 : forall v E,
-      s_value v -> s_eval_context E -> s_eval_context (s_ctx_app2 v E).
-
-(* TODO: santity check theorem *)
+      s_value v -> s_eval_context E ->
+      s_eval_context (s_ctx_app2 v E).
 
 Inductive s_context : ctx -> Prop :=
   | s_context_hole : s_context s_ctx_hole
   | s_context_if : forall C e1 e2,
-      s_context C -> s_term e1 -> s_term e2 -> s_context (s_ctx_if C e1 e2)
+      s_context C -> s_term e1 -> s_term e2 ->
+      s_context (s_ctx_if C e1 e2)
   | s_context_app1 : forall C e,
-      s_context C -> s_term e -> s_context (s_ctx_app1 C e)
+      s_context C -> s_term e ->
+      s_context (s_ctx_app1 C e)
   | s_context_app2 : forall v C,
-      s_value v -> s_context C -> s_context (s_ctx_app2 v C)
+      s_value v -> s_context C ->
+      s_context (s_ctx_app2 v C)
   | s_context_abs : forall L T C,
-      (forall x, x \notin L -> s_context (s_ctx_open_var C x)) ->
+      (forall x, x \notin L -> s_context (s_ctx_open_ee_var C x)) ->
       (s_type T) ->
       s_context (s_ctx_abs T C)
   | s_context_if_true : forall e1 C e3,
-      s_term e1 -> s_context C -> s_term e3 -> s_context (s_ctx_if_true e1 C e3)
+      s_term e1 -> s_context C -> s_term e3 ->
+      s_context (s_ctx_if_true e1 C e3)
   | s_context_if_false : forall e1 e2 C,
-      s_term e1 -> s_term e2 -> s_context C -> s_context (s_ctx_if_false e1 e2 C).
-
-(* TODO: santity check theorem *)
+      s_term e1 -> s_term e2 -> s_context C ->
+      s_context (s_ctx_if_false e1 e2 C).
 
 (* typing for contexts *)
 
-Inductive s_context_typing : ctx -> env -> typ -> env -> typ -> Prop :=
+Inductive s_context_typing (* |- C : G |- s ~> G' |- s' *)
+  : ctx -> env_term -> typ -> env_term -> typ -> Prop :=
   | s_context_typing_hole : forall G_hole s_hole G,
       s_ok G_hole -> s_ok G -> extends G_hole G -> 
       s_type s_hole ->
-      s_context_typing s_ctx_hole G_hole s_hole G T_hole
+      s_context_typing s_ctx_hole G_hole s_hole G s_hole
   | s_context_typing_if : forall C G_hole s_hole G e2 e3 s,
       s_context_typing C G_hole s_hole G s_typ_bool ->
       s_typing G e2 s -> s_typing G e3 s ->
       s_context_typing (s_ctx_if C e2 e3) G_hole s_hole G s
   | s_context_typing_app1 : forall C G_hole s_hole G e s s',
-      s_context_typing C G_hole s_hole G (s_type_arrow s s') ->
+      s_context_typing C G_hole s_hole G (s_typ_arrow s s') ->
       s_typing G e s ->
       s_context_typing (s_ctx_app1 C e) G_hole s_hole G s'
   | s_context_typing_app2 : forall C G_hole s_hole G e s s',
-      s_typing G e (s_type_arrow s s') ->
+      s_typing G e (s_typ_arrow s s') ->
       s_context_typing C G_hole s_hole G s ->
       s_context_typing (s_ctx_app2 e C) G_hole s_hole G s'
   | s_context_typing_abs : forall L C G_hole s_hole G s s',
-      (forall x, x \notin L ->
-        s_context_typing (s_ctx_open_var C x) G_hole s_hole (G & x ~ s) s') ->
-      s_type T -> (* XXX: Not sure if this check is necessary. *)
-      s_context_typing (s_ctx_abs s C) G_hole s_hole G (s_type_arrow s s')
+      (forall x, x \notin L -> s_context_typing (s_ctx_open_ee_var C x)
+                                                G_hole s_hole
+                                                (G & x ~ s) s') ->
+      s_type s -> (* XXX: Not sure if this check is necessary. *)
+      s_context_typing (s_ctx_abs s C) G_hole s_hole G (s_typ_arrow s s')
   | s_context_typing_if_true : forall C G_hole s_hole G e1 e3 s,
-      s_typing G e1 s_type_bool ->
-      (* TODO: Go back and s/s_type/s_typ/g *)
+      s_typing G e1 s_typ_bool ->
       s_context_typing C G_hole s_hole G s ->
       s_typing G e3 s ->
       s_context_typing (s_ctx_if_true e1 C e3) G_hole s_hole G s
   | s_context_typing_if_false : forall C G_hole s_hole G e1 e2 s,
-      s_typing G e1 s_type_bool -> s_typing G e2 s ->
+      s_typing G e1 s_typ_bool -> s_typing G e2 s ->
       s_context_typing C G_hole s_hole G s ->
       s_context_typing (s_ctx_if_false e1 e2 C) G_hole s_hole G s.
-
-(* TODO: santity check theorem *)
 
 (* reduction *)
 
@@ -148,17 +142,14 @@ Inductive s_red_base : trm -> trm -> Prop :=
   | s_red_if_false : forall e1 e2,
       s_term e1 -> s_term e2 ->
       s_red_base (s_trm_if s_trm_false e1 e2) e2
-  | s_red_app : forall e v T1,
-      s_value (s_trm_abs T1 e) -> s_value v ->
-      s_red_base (s_trm_app (s_trm_abs T1 e) v) (s_open_ee_var e v).
-
-(* TODO: santity check theorem *)
-(* TODO: Requires definition of plug *)
+  | s_red_app : forall e v s,
+      s_value (s_trm_abs s e) -> s_value v ->
+      s_red_base (s_trm_app (s_trm_abs s e) v) (s_open_ee e v).
 
 Inductive s_red : trm -> trm -> Prop :=
   | s_red_ctx : forall E e e',
       s_red_base e e' -> s_eval_context E ->
-      s_red (s_plug E e) (s_plug E e').
+      s_red (plug E e) (plug E e').
 
 Inductive s_red_star : trm -> trm -> Prop :=
   | s_red_refl : forall e, s_term e -> s_red_star e e
@@ -169,46 +160,33 @@ Inductive s_eval : trm -> trm -> Prop :=
   | s_eval_red : forall e v,
       s_red_star e v -> s_value v -> s_eval e v.
 
-(* TODO: I am here *)
-
 (* contextual equivalence *)
 
-Definition s_ctx_approx (G : env) (e1 e2 : trm) (T : typ) :=
-  s_typing G e1 T /\ s_typing G e2 T /\
+Definition s_ctx_approx (G : env_term) (e1 e2 : trm) (s : typ) :=
+  s_typing G e1 s /\ s_typing G e2 s /\
   forall C v,
-    s_context_typing C G T empty s_typ_bool ->
-    s_eval (s_plug C e1) v ->
-    s_eval (s_plug C e2) v.
+    s_context_typing C G s empty s_typ_bool ->
+    s_eval (plug C e1) v ->
+    s_eval (plug C e2) v.
 
-Definition ctx_equiv (G : env) (e1 e2 : trm) (T : type) :=
-  ctx_approx G e1 e2 T /\ ctx_approx G e2 e1 T.
+Definition s_ctx_equiv (G : env_term) (e1 e2 : trm) (s : typ) :=
+  s_ctx_approx G e1 e2 s /\ s_ctx_approx G e2 e1 s.
 
 (* CIU equivalence *)
 
-Definition substitution := LibEnv.env trm.
+Inductive s_subst_satisfies : subst_term -> env_term -> Prop :=
+| s_subst_satisfies_empty : s_subst_satisfies empty empty
+| s_subst_satisfies_extend : forall g G x v s,
+    s_subst_satisfies g G -> x # G -> s_typing empty v s ->
+    s_subst_satisfies (g & x ~ v) (G & x ~ s).
 
-Definition subst_satisfies g G :=
-  forall x v T, binds x v g -> value v /\ binds x T G /\ typing empty v T.
-
-Fixpoint apply_subst (g : substitution) (e : trm) :=
-  match e with
-  | trm_bvar n => trm_bvar n
-  | trm_fvar x => match get x g with None => trm_fvar x
-                    | Some v => v end
-  | trm_true => trm_true
-  | trm_false => trm_false
-  | trm_abs T e => trm_abs T (apply_subst g e)
-  | trm_if e1 e2 e3 => trm_if (apply_subst g e1)
-                              (apply_subst g e2)
-                              (apply_subst g e3)
-  | trm_app e1 e2 => trm_app (apply_subst g e1)
-                            (apply_subst g e2)
-  end.
-
-Definition ciu_approx (G : env) (e1 e2 : trm) (T : type) :=
-  typing G e1 T /\ typing G e2 T /\
+Definition s_ciu_approx (G : env_term) (e1 e2 : trm) (s : typ) :=
+  s_typing G e1 s /\ s_typing G e2 s /\
   forall E g v,
-    eval_context E -> context_typing E empty T empty type_bool ->
-    subst_satisfies g G ->
-    eval (plug E (apply_subst g e1)) v ->
-    eval (plug E (apply_subst g e2)) v.
+    s_eval_context E -> s_context_typing E empty s empty s_typ_bool ->
+    s_subst_satisfies g G ->
+    s_eval (plug E (subst_ee g e1)) v ->
+    s_eval (plug E (subst_ee g e2)) v.
+
+Definition s_ciu_equiv (G : env_term) (e1 e2 : trm) (s : typ) :=
+  s_ciu_approx G e1 e2 s /\ s_ciu_approx G e2 e1 s.
